> The following code fragment implements Horner's rule for evaluating a polynomial
>
> $$
> \begin{aligned}
> P(x) & = \sum_{k = 0}^n a_k x^k \\\\
>      & = a_0 + x(a_1 + x (a_2 + \cdots + x(a_{n - 1} + x a_n) \cdots)),
> \end{aligned}
> $$
>
> given the coefficients $a_0, a_1, \ldots, a_n$ and a value of $x$:
>
> ```cpp
> y = 0
> for i = n downto 0
>     y = a[i] + x * y
> ```
>
> **a.** In terms of $\Theta$-notation, what is the running time of this code fragment for Horner's rule?
>
> **b.** Write pseudocode to implement the naive polynomial-evaluation algorithm that computes each term of the polynomial from scratch. What is the running time of this algorithm? How does it compare to Horner's rule
>
> **c.** Consider the following loop invariant: At the start of each iteration of the **for** loop of lines 2-3,
>
> $$y = \sum_{k = 0}^{n - (i + 1)} a_{k + i + 1} x^k.$$
>
> Interpret a summation with no terms as equaling $0$. Following the structure of the loop invariant proof presented in this chapter, use this loop invariant to show that, at termination, $y = \sum_{k = 0}^n a_k x^k$.
>
> **d.** Conclude by arguing that the given code fragment correctly evaluates a polynomial characterized by the coefficients $a_0, a_1, \ldots, a_n$.

**a.** $\Theta(n)$.

**b.**

```cpp
NAIVE-HORNER()
    y = 0
    for k = 0 to n
        temp = 1
        for i = 1 to k
            temp = temp * x
            y = y + a[i] * m
```

The running time is $\Theta(n^2)$, because of the nested loop. It is obviously slower.

**c.** **Initialization:** It is pretty trivial, since the summation has no terms which implies $y = 0$.

**Maintenance:** By using the loop invariant, in the end of the $i$-the iteration, we have

$$
\begin{aligned}
y & = a_i + x \sum_{k = 0}^{n - (i + 1)} a_{k + i + 1} x^k \\\\
  & = a_i x^0 + \sum_{k = 0}^{n - i - 1} a_{k + i + 1} x^{k + 1} \\\\
  & = a_i x^0 \sum_{k = 1}^{n - i} a_{k + i} x^k \\\\
  & = \sum_{k = 0}^{n - i} a_{k + i} x^k.
\end{aligned}
$$

**Termination:** The loop terminates at $i = -1$. If we substitute,

$$y = \sum_{k = 0}^{n - i - 1} a_{k + i + 1} x^k = \sum_{k = 0}^n a_k x^k.$$

**d.** The invariant of the loop is a sum that equals a polynomial with the given coefficients.
