> Let $b_n$ denote the number of different binary trees with $n$ nodes. In this problem, you will find a formula for $b_n$, as well as an asymptotic estimate.
>
> **a.** Show that $b_0 = 1$ and that, for $n \ge 1$,
>
> $$b_n = \sum_{k = 0}^{n - 1} b_k b_{n - 1 - k}.$$
>
> **b.** Referring to Problem 4-4 for the definition of a generating function, let $B(x)$ be the generating function
>
> $$B(x) = \sum_{n = 0}^\infty b_n x^n.$$
>
> Show that $B(x) = xB(x)^2 + 1$, and hence one way to express $B(x)$ in closed form is
>
> $$B(x) = \frac{1}{2x} (1 - \sqrt{1 - 4x}).$$
>
> The **_Taylor expansion_** of $f(x)$ around the point $x = a$ is given by
>
> $$f(x) = \sum_{k = 0}^\infty \frac{f^{(k)}(a)}{k!} (x - a)^k,$$
>
> where $f^{(k)}(x)$ is the $k$th derivative of $f$ evaluated at $x$.
>
> **c.** Show that
>
> $$b_n = \frac{1}{n + 1} \binom{2n}{n}$$
>
> (the $n$th **_Catalan number_**) by using the Taylor expansion of $\sqrt{1 - 4x}$ around $x = 0$. (If you wish, instead of using the Taylor expansion, you may use the generalization of the binomial expansion (C.4) to nonintegral exponents $n$, where for any real number $n$ and for any integer $k$, we interpret $\binom{n}{k}$ to be $n(n - 1) \cdots (n - k + 1) / k!$ if $k \ge 0$, and $0$ otherwise.)
>
> **d.** Show that
>
> $$b_n = \frac{4^n}{\sqrt{\pi}n^{3 / 2}} (1 + O(1 / n)).$$

**a.** A root with two subtree.

**b.**

$$
\begin{aligned}
B(x)^2 & = (b_0 x^0 + b_1 x^1 + b_2 x^2 + \cdots)^2 \\\\
       & = b_0^2 x^0 + (b_0 b_1 + b_1 b_0) x^1 + (b_0 b_2 + b_1 b_1 + b_2 b_0) x^2 + \cdots \\\\
       & = \sum_{k = 0}^0 b_k b_{0 - k} x^0 + \sum_{k = 0}^1 b_k b_{1 - k} x^1 + \sum_{k = 0}^2 b_k b_{2 - k} x^2 + \cdots
\end{aligned}
$$

$$
\begin{aligned}
xB(x)^2 + 1 & = 1 + \sum_{k = 0}^0 b_k b_{1 - 1 - k} x^1 + \sum_{k = 0}^2 b_k b_{2-1 - k} x^3 + \sum_{k = 0}^2 b_k b_{3-1 - k} x^2 + \cdots \\\\
            & = 1 + b_1 x^1 + b_2 x^2 + b_3 x^3 + \cdots \\\\
            & = b_0 x^0 + b_1 x^1 + b_2 x^2 + b_3 x^3 + \cdots \\\\
            & = \sum_{n = 0}^\infty b_n x^n \\\\
            & = B(x).
\end{aligned}
$$

$$
\begin{aligned}
x B(x)^2 + 1 & = x \cdot \frac{1}{4x^2} (1 + 1 - 4x - 2\sqrt{1 - 4x}) + 1 \\\\
             & = \frac{1}{4x} (2 - 2\sqrt{1 - 4x}) - 1 + 1 \\\\
             & = \frac{1}{2x} (1 - \sqrt{1 - 4x}) \\\\
             & = B(x).
\end{aligned}
$$

**c.** Let $f(x) = \sqrt{1 - 4x}$, the numerator of the derivative is

$$
\begin{aligned}
2 \cdot (1 \cdot 2) \cdot (3 \cdot 2) \cdot (5 \cdot 2) \cdots
    & = 2^k \cdot \prod_{i = 0}^{k - 2} (2k + 1) \\\\
    & = 2^k \cdot \frac{(2(k - 1))!}{2^{k - 1}(k - 1)!} \\\\
    & = \frac{2(2(k - 1))!}{(k - 1)!}.
\end{aligned}
$$

$$f(x) = 1 - 2x - 2x^2 - 4 x^3 - 10x^4 - 28x^5 - \cdots.$$

The coefficient is $\frac{2(2(k - 1))!}{k!(k - 1)!}$.

$$
\begin{aligned}
B(x) & = \frac{1}{2x}(1 - f(x)) \\\\
     & = 1 + x + 2x^2 + 5x^3 + 14x^4 + \cdots \\\\
     & = \sum_{n = 0}^\infty \frac{(2n)!}{(n + 1)!n!} x \\\\
     & = \sum_{n = 0}^\infty \frac{1}{n + 1} \frac{(2n)!}{n!n!} x \\\\
     & = \sum_{n = 0}^\infty \frac{1}{n + 1} \binom{2n}{n} x.
\end{aligned}
$$

$$b_n = \frac{1}{n + 1} \binom{2n}{n}.$$

**d.**

$$
\begin{aligned}
b_n & =       \frac{1}{n + 1} \frac{(2n)!}{n!n!} \\\\
    & \approx \frac{1}{n + 1} \frac{\sqrt{4 \pi n}(2n / e)^{2n}}{2 \pi n (n / e)^{2n}} \\\\
    & =       \frac{1}{n + 1} \frac{4^n}{\sqrt{\pi n} } \\\\
    & =       (\frac{1}{n} + (\frac{1}{n + 1} - \frac{1}{n})) \frac{4^n}{\sqrt{\pi n}} \\\\
    & =       (\frac{1}{n} - \frac{1}{n^2 + n}) \frac{4^n}{\sqrt{\pi n}} \\\\
    & =       \frac{1}{n} (1 - \frac{1}{n + 1}) \frac{4^n}{\sqrt{\pi n}} \\\\
    & =       \frac{4^n}{\sqrt{\pi}n^{3 / 2}} (1 + O(1 / n)).
\end{aligned}
$$
