> **a.** Rank the following functions by order of growth; that is, find an arrangement $g_1, g_2, \ldots , g_{30}$ of the functions $g_1 = \Omega(g_2), g_2 = \Omega(g_3), \ldots, g_{29} = \Omega(g_{30})$. Partition your list into equivalence classes such that functions $f(n)$ and $g(n)$ are in the same class if and only if $f(n) = \Theta(g(n))$.
>
> $$
> \begin{array}{cccccc}
> \lg(\lg^{^\*}n) \quad & \quad 2^{\lg^\*n} \quad & \quad (\sqrt 2)^{\lg n} \quad & \quad n^2 \quad & \quad n! \quad & \quad (\lg n)! \\\\
> (\frac{3}{2})^n \quad & \quad n^3 \quad & \quad \lg^2 n \quad & \quad \lg(n!) \quad & \quad 2^{2^n} \quad & \quad n^{1/\lg n} \\\\
> \lg\lg n \quad & \quad \lg^\* n \quad & \quad n\cdot 2^n \quad & \quad n^{\lg\lg n} \quad & \quad \lg n \quad & \quad 1 \\\\
> 2^{\lg n} \quad & \quad (\lg n)^{\lg n} \quad & \quad e^n \quad & \quad 4^{\lg n}  \quad & \quad (n + 1)! \quad & \quad \sqrt{\lg n} \\\\
> \lg^\*(\lg n) \quad & \quad 2^{\sqrt{2\lg n}} \quad & \quad n \quad & \quad 2^n \quad & \quad n\lg n \quad & \quad 2^{2^{n + 1}}
> \end{array}
> $$
>
> **b.** Give an example of a single nonnegative function $f(n)$ such that for all functions $g_i(n)$ in part (1), $f(n)$ is neither $O(g_i(n))$ nor $\Omega(g_i(n))$.

**a.** Here is the ordering, where functions on the same line are in the same equivalence class, and those higher on the page are $\Omega$ of those below them:

$$
\begin{array}{ll}
2^{2^{n + 1}}                      & \\\\
2^{2^n}                            & \\\\
(n + 1)!                           & \\\\
n!                                 & \text{see justification 7} \\\\
e^n                                & \text{see justification 1} \\\\
n\cdot 2^n                         & \\\\
2^n                                & \\\\
(3 / 2)^n                          & \\\\
(\lg n)^{\lg n} = n^{\lg\lg n}     & \text{see identity 1} \\\\
(\lg n)!                           & \text{see justifications 2, 8} \\\\
n^3                                & \\\\
n^2 = 4^{\lg n}                    & \text{see identity 2} \\\\
n\lg n \text{ and } \lg(n!)        & \text{see justification 6} \\\\
n = 2^{\lg n}                      & \text{see identity 3} \\\\
(\sqrt 2)^{\lg n}(= \sqrt n)       & \text{see identity 6, justification 3} \\\\
2^{\sqrt{2\lg n}}                  & \text{see identity 5, justification 4}\\\\
\lg^2 n                            & \\\\
\ln n                              & \\\\
\sqrt{\lg n}                       & \\\\
\ln\ln n                           & \text{see justification 5} \\\\
2^{\lg^\*n}                        & \\\\
\lg^\*n \text{ and } \lg^\*(\lg n) & \text{see identity 7} \\\\
\lg(\lg^\*)n                       & \\\\
n^{1 / \lg n}(= 2) \text{ and } 1  & \text{see identity 4}
\end{array}
$$

Much of the ranking is based on the following properties:

- Exponential functions grow faster than polynomial functions, which grow faster than polylogarithmic functions.
- The base of a logarithm doen't matter asymptotically, but the base of an exponential and the degree of a polynomial do matter.

We have the following $\textit{identities}$:

1. $(\lg n)^{\lg n} = n^{\lg\lg n}$ because $a^{\log_b c} = c^{\log_b a}$.
2. $4^{\lg n} = n^2$ because $a^{\log_b c} = c^{\log_b a}$.
3. $2^{\lg n} = n$.
4. $2 = n^{1 / \lg n}$ by raising identity 3 to the power $1 / \lg n$.
5. $2^{\sqrt{2\lg n}} = n^{\sqrt{2 / \lg n}}$ by raising identity 4 to the power $\sqrt{2\lg n}$.
6. $(\sqrt 2)^{\lg n} = \sqrt n$ because $(\sqrt 2)^{\lg n} = 2^{(1 / 2)\lg n} = 2^{\lg\sqrt n} = \sqrt n$.
7. $\lg^\*(\lg n) = (\lg^\*n) - 1$.

The following $\textit{justifications}$ explain some of the rankings:

1. $e^n = 2^n(e / 2)^n = \omega(n2^n)$, since $(e/2)^n = \omega(n)$.
2. $(\lg n) \ne \omega(n^3)$ by taking logs: $\lg(\lg n) \ne \Theta(\lg n\lg\lg n)$ by Stirling's approximation, $\lg(n^3) = 3\lg n$. $\lg\lg n = \omega(3)$.
3. $(\sqrt 2)^{\lg n} = \omega(2^{\sqrt{2\lg n}})$ by taking logs: $\lg(\sqrt 2)^{\lg n} = (1 / 2)\lg n,\lg 2^{\sqrt{2\lg n}}  =  \sqrt{2\lg n}$. $(1 / 2)\lg n = \omega(\sqrt{2\lg n})$.
4. $2^{\sqrt{2\lg n}} = \omega(\lg^2 n)$ by taking logs: $\lg 2^{\sqrt{2\lg n}} = \sqrt{2\lg n},\lg\lg^2n = 2\lg\lg n$. $\sqrt{2\lg n} = \omega(2\lg\lg n)$.
5. $\ln\ln n = \omega(2^{\lg^\*n})$ by taking logs: $\lg 2^{\lg^\* n} = \lg^\*n$. $\lg\ln\ln n = \omega(\lg^\*n)$.
6. $\lg(n!) = \Theta(n\lg n)$ (equation $\text{(3.18)}$).
7. $n \ne \Theta(n^{n + 1}e^{-n})$ by dropping constants and low-order terms in equation $\text{(3.17)}$.
8. $(\lg n) \ne \Theta((\lg n)^{\lg n + 1 / 2} e^{-\lg n}$ by substituting $\lg n$ for $n$ in the previous justification. $(\lg n) \ne \Theta((\lg n)^{\lg n + 1 / 2}n^{-\lg e})$ because $a^{\log_b c} = c^{\log_b a}$.

**b.** The following $f(n)$ is nonnegative, and for all functions $g_i(n)$ in part (1), $f(n)$ is neither $O(g_i(n))$ nor $\Omega(g_i(n))$.

$$
f(n) =
\begin{cases} 2^{2^{n + 2}} & \text{if $n$ is even}, \\\\
                          0 & \text{if $n$ is odd}.
\end{cases}
$$
